libcrux-ml-kem/proofs/fstar/extraction/Libcrux_ml_kem.Vector.Avx2.Serialize.fst
@@ -3,15 +3,105 @@ module Libcrux_ml_kem.Vector.Avx2.Serialize
 open Core
 open FStar.Mul
 
+module _ = Tactics.Utils
+module _ = Tactics.Seq
+module _ = BitVecEq
+
 let _ =
   (* This module has implicit dependencies, here we make them explicit. *)
   (* The implicit dependencies arise from typeclasses instances. *)
   let open Libcrux_ml_kem.Vector.Portable in
   ()
 
+open BitVec.Intrinsics {mk_bv}
+
+// 2:29 PM
+// let shift_lsb_to_msb = mm256_set_epi16(
+//         8,
+//         9,
+//         10,
+//         11,
+//         12,
+//         13,
+//         14,
+//         15,
+//         8,
+//         9,
+//         10,
+//         11,
+//         12,
+//         13,
+//         14,
+//         15,
+//     );
+
+
+let specialized_mm256_mullo_epi16 (a: bit_vec 256): bit_vec 256 =
+  mk_bv (fun i -> 
+    let nth_bit = i % 16 in
+    let nth_i16 = i / 16 in
+    let shift = if nth_i16 >= 8 then 23 - nth_i16 else 15 - nth_i16 in
+    if nth_bit >= shift then a (i - shift) else 0
+  )
+
+let mm256_srli_epi16 (shift: nat {shift <= 16}) (vec: bit_vec 256): bit_vec 256
+  = mk_bv (fun i -> // are `i` and `i + shift` position of the same 16-bits integer?
+                 let nth_bit = i % 16 in
+                 if nth_bit < 16 - shift then vec (i + shift) else 0
+                 // if i / 16 = (i + shift) / 16
+                 // then vec (i + shift)
+                 // else 0
+                 )
+
+open FStar.Tactics.V2
+open Tactics.Utils
+
+let rw_get_bit_cast #t #u
+  (x: int_t t) (nth: usize)
+  : Lemma (requires v nth < bits u /\ v nth < bits u)
+          (ensures eq2 #bit (get_bit (cast_mod #t #u x) nth) (if v nth < bits t then get_bit x nth else 0))
+          [SMTPat (get_bit (cast_mod #t #u x) nth)]
+  = ()
+
+let rw_get_bit_shr #t #u (x: int_t t) (y: int_t u) (i: usize {v i < bits t})
+  : Lemma (requires v y >= 0 /\ v y < bits t)
+          (ensures eq2 #bit (get_bit (x >>! y) i )
+                (if v i < bits t - v y
+                    then get_bit x (mk_int (v i + v y))
+                    else if signed t
+                         then get_bit x (mk_int (bits t - 1))
+                         else 0))
+  = ()
+
+let mm256_set_epi16 (x0 x1 x2 x3 x4 x5 x6 x7 x8 x9 x10 x11 x12 x13 x14 x15: i16)
+  : bit_vec 256
+  = mk_bv (fun i ->
+      let offset = i % 16 in
+      match i / 16 with
+      |  0 -> get_bit x15 (sz offset)
+      |  1 -> get_bit x14 (sz offset)
+      |  2 -> get_bit x13 (sz offset)
+      |  3 -> get_bit x12 (sz offset)
+      |  4 -> get_bit x11 (sz offset)
+      |  5 -> get_bit x10 (sz offset)
+      |  6 -> get_bit x9 (sz offset)
+      |  7 -> get_bit x8 (sz offset)
+      |  8 -> get_bit x7 (sz offset)
+      |  9 -> get_bit x6 (sz offset)
+      | 10 -> get_bit x5 (sz offset)
+      | 11 -> get_bit x4 (sz offset)
+      | 12 -> get_bit x3 (sz offset)
+      | 13 -> get_bit x2 (sz offset)
+      | 14 -> get_bit x1 (sz offset)
+      | 15 -> get_bit x0 (sz offset)
+    )
+
+
 let deserialize_1_ (bytes: t_Slice u8) =
+  assume (Seq.length bytes == 2);
   let coefficients:Libcrux_intrinsics.Avx2_extract.t_Vec256 =
-    Libcrux_intrinsics.Avx2_extract.mm256_set_epi16 (cast (bytes.[ sz 1 ] <: u8) <: i16)
+    // WARNING: using `BitVec.Intrinsics.mm256_set_epi16` here for now, we need to bind it in extract_avx2.rs
+    mm256_set_epi16 (cast (bytes.[ sz 1 ] <: u8) <: i16)
       (cast (bytes.[ sz 1 ] <: u8) <: i16) (cast (bytes.[ sz 1 ] <: u8) <: i16)
       (cast (bytes.[ sz 1 ] <: u8) <: i16) (cast (bytes.[ sz 1 ] <: u8) <: i16)
       (cast (bytes.[ sz 1 ] <: u8) <: i16) (cast (bytes.[ sz 1 ] <: u8) <: i16)
@@ -21,16 +111,52 @@ let deserialize_1_ (bytes: t_Slice u8) =
       (cast (bytes.[ sz 0 ] <: u8) <: i16) (cast (bytes.[ sz 0 ] <: u8) <: i16)
       (cast (bytes.[ sz 0 ] <: u8) <: i16)
   in
-  let shift_lsb_to_msb:Libcrux_intrinsics.Avx2_extract.t_Vec256 =
-    Libcrux_intrinsics.Avx2_extract.mm256_set_epi16 (1s <<! 8l <: i16) (1s <<! 9l <: i16)
-      (1s <<! 10l <: i16) (1s <<! 11l <: i16) (1s <<! 12l <: i16) (1s <<! 13l <: i16)
-      (1s <<! 14l <: i16) (-32768s) (1s <<! 8l <: i16) (1s <<! 9l <: i16) (1s <<! 10l <: i16)
-      (1s <<! 11l <: i16) (1s <<! 12l <: i16) (1s <<! 13l <: i16) (1s <<! 14l <: i16) (-32768s)
-  in
+  // let shift_lsb_to_msb:Libcrux_intrinsics.Avx2_extract.t_Vec256 =
+  //   Libcrux_intrinsics.Avx2_extract.mm256_set_epi16 (1s <<! 8l <: i16) (1s <<! 9l <: i16)
+  //     (1s <<! 10l <: i16) (1s <<! 11l <: i16) (1s <<! 12l <: i16) (1s <<! 13l <: i16)
+  //     (1s <<! 14l <: i16) (-32768s) (1s <<! 8l <: i16) (1s <<! 9l <: i16) (1s <<! 10l <: i16)
+  //     (1s <<! 11l <: i16) (1s <<! 12l <: i16) (1s <<! 13l <: i16) (1s <<! 14l <: i16) (-32768s)
+  // in
   let coefficients_in_msb:Libcrux_intrinsics.Avx2_extract.t_Vec256 =
-    Libcrux_intrinsics.Avx2_extract.mm256_mullo_epi16 coefficients shift_lsb_to_msb
+    // Libcrux_intrinsics.Avx2_extract.
+    specialized_mm256_mullo_epi16 coefficients 
+    //shift_lsb_to_msb
   in
-  Libcrux_intrinsics.Avx2_extract.mm256_srli_epi16 15l coefficients_in_msb
+  // Libcrux_intrinsics.Avx2_extract.
+  let result = mm256_srli_epi16 15 coefficients_in_msb in
+  assert (forall (i: nat {i < 16}). result (i * 16) == bit_vec_of_int_t_array #_ #2 bytes 8 i) by (
+    Tactics.Utils.prove_forall_nat_pointwise (fun _ ->
+      norm [iota; primops; delta_only [`%cast; `%cast_tc_integers]];
+      l_to_r [`rw_get_bit_cast];
+      let light_norm () = norm [ iota; primops; zeta_full
+           ; delta_only [`%bit_vec_of_int_t_array;`%bits;`%Lib.IntTypes.bits]
+           ; delta_namespace ["FStar"]
+      ] in
+      light_norm ();
+      Tactics.Seq.norm_index ();
+      l_to_r[`rw_get_bit_cast; `bit_vec_to_int_t_lemma; `get_bit_shr];
+      Tactics.MachineInts.(transform norm_machine_int_term);
+      light_norm ();
+      norm [primops; iota; zeta_full; delta_only [
+        `%Libcrux_intrinsics.Avx2_extract.mm_movemask_epi8;
+        `%BitVec.Intrinsics.mm_movemask_epi8;
+      ]];
+      l_to_r [`rw_get_bit_cast; `bit_vec_to_int_t_lemma; `get_bit_shr];
+      let _ = rewrite_lhs () in
+      flip ();
+      trefl ();
+      l_to_r [`rw_get_bit_shr];
+      Tactics.MachineInts.(transform norm_machine_int_term);
+      l_to_r [`rw_get_bit_cast; `bit_vec_to_int_t_lemma; `get_bit_shr];
+      light_norm ();
+      norm [primops; iota; zeta_full; delta_namespace ["Libcrux_intrinsics.Avx2_extract";"BitVec.Intrinsics"; implode_qn (cur_module ()); "FStar"]];
+      dump' "Goal:";
+      smt_sync ();
+      dump' "Success";
+      smt ()
+    )
+  );
+  result
 
 let deserialize_10_ (bytes: t_Slice u8) =
   let shift_lsbs_to_msbs:Libcrux_intrinsics.Avx2_extract.t_Vec256 =
@@ -209,39 +335,6 @@ let deserialize_5_ (bytes: t_Slice u8) =
         Libcrux_intrinsics.Avx2_extract.t_Vec256)
   in
   Libcrux_intrinsics.Avx2_extract.mm256_srli_epi16 11l coefficients
-
-open FStar.Tactics.V2
-open Tactics.Utils
-
-// let _ = get_bit_cast
-
-let rw_get_bit_cast #t #u
-  (x: int_t t) (nth: usize)
-  : Lemma (requires v nth < bits u /\ v nth < bits u)
-          (ensures eq2 #bit (get_bit (cast_mod #t #u x) nth) (if v nth < bits t then get_bit x nth else 0))
-          [SMTPat (get_bit (cast_mod #t #u x) nth)]
-  = ()
-
-let rw_get_bit_shr #t #u (x: int_t t) (y: int_t u) (i: usize {v i < bits t})
-  : Lemma (requires v y >= 0 /\ v y < bits t)
-          (ensures eq2 #bit (get_bit (x >>! y) i )
-                (if v i < bits t - v y
-                    then get_bit x (mk_int (v i + v y))
-                    else if signed t
-                         then get_bit x (mk_int (bits t - 1))
-                         else 0))
-  = ()
-
-// val bit_vec_to_int_t_lemma
-//     #t (d: num_bits t) (bv: bit_vec d)
-//     i
-//   : Lemma (eq2 #bit (get_bit (bit_vec_to_int_t d bv) (sz i)) (bv i))
-
-// val bit_vec_to_int_t_lemma2
-//     #t (d: num_bits t) (bv: bit_vec d)
-//     i
-//   : Lemma (eq2 (get_bit (bit_vec_to_int_t d bv) (sz i)) (bv i))
-
 
 #push-options "--compat_pre_core 0"
 #push-options "--z3rlimit 90"
